symboles preuve -> ascii

proof_Isabelle/sync-mod/SyncMod.thy
@@ -19,63 +19,64 @@ locale k_mod = fixes k :: nat
 begin
 
 definition SyncMod_initState where 
-"SyncMod_initState p st \<equiv> x st = k \<and> (\<not> forc st) \<and> \<not> fire st"
+"SyncMod_initState p st == x st = k & (~ forc st) & ~ fire st"
 
 definition concordant where
-"concordant msgs v \<equiv> \<exists>p. msgs p = Content (Val v) \<and> (\<forall>q vv. msgs q = Content (Val vv) \<longrightarrow> vv = v)"
+"concordant msgs v == EX p. msgs p = Content (Val v) & (ALL q vv. msgs q = Content (Val vv) --> vv = v)"
 
 definition ready_fire where
-"ready_fire msgs \<equiv> \<forall>p. msgs p = Void \<or> msgs p = Content (Val (k-1))"
+"ready_fire msgs == ALL p. msgs p = Void \<or> msgs p = Content (Val (k-1))"
 
 definition ready_force where
-"ready_force msgs ss \<equiv> (\<not> forc ss) \<and> (\<forall>p. msgs p \<noteq> Content (Val (k-1))) \<and> 
-(\<exists>p q v1 v2. msgs p = Content (Val v1) \<and> msgs q = Content (Val v2) \<and> v1 \<noteq> v2)"
+"ready_force msgs ss == (~ forc ss) \<and> (ALL p. msgs p ~= Content (Val (k-1))) \<and> 
+(EX p q v1 v2. msgs p = Content (Val v1) \<and> msgs q = Content (Val v2) & v1 ~= v2)"
 
-definition SyncMod_nextState :: "Proc \<Rightarrow> pstate \<Rightarrow> (Proc \<Rightarrow> SendVal message) \<Rightarrow> pstate \<Rightarrow> bool" where
-"SyncMod_nextState p ss msgs st \<equiv>
+definition SyncMod_nextState :: "Proc => pstate => (Proc => SendVal message) => pstate => bool" where
+"SyncMod_nextState p ss msgs st ==
     fire st = (ready_fire msgs | fire ss) &
     (if ready_force msgs ss then
         x st = k-1 & forc st
         else forc ss = forc st & (
-            if EX v. concordant msgs v then x st = (Suc (Eps (%v. concordant msgs v))) mod k else x st = 0))"
+            if EX v. concordant msgs v then x st = (Suc (SOME v. concordant msgs v)) mod k else x st = 0))"
         (*"if x st = 0 then
-            \<forall>v. concordant msgs v \<longrightarrow> v = k - 1 else
+            ALL v. concordant msgs v --> v = k - 1 else
             concordant msgs ((x st - 1) mod k)) \<and> (x st) mod k = x st)"*)
 
 definition SyncMod_sendMsg where
-"SyncMod_sendMsg p q st \<equiv> if x st = k then Nope else Val (x st)"
+"SyncMod_sendMsg p q st == if x st = k then Nope else Val (x st)"
 
 definition SyncMod_commPerRd where
-"SyncMod_commPerRd HO \<equiv> True"
+"SyncMod_commPerRd HO == True"
 
 definition xi_nek where 
-"xi_nek HO xi \<equiv> \<forall>p n. xi \<in> HO n p"
+"xi_nek HO xi == ALL p n. xi : HO n p"
 
 definition SyncMod_commGlobal where
-"SyncMod_commGlobal HO \<equiv> \<exists>xi. xi_nek HO xi"
+"SyncMod_commGlobal HO == EX xi. xi_nek HO xi"
 
 definition SyncMod_commSchedule where
-"SyncMod_commSchedule sched \<equiv> \<exists>n. sched n = UNIV"
+"SyncMod_commSchedule sched == EX n. sched n = UNIV"
 
 definition SyncMod_HOMachine where
-"SyncMod_HOMachine \<equiv> \<lparr>
-    CinitState = (\<lambda> p st crd. SyncMod_initState p st),
+"SyncMod_HOMachine == \<lparr>
+    CinitState = (% p st crd. SyncMod_initState p st),
     sendMsg = SyncMod_sendMsg,
-    CnextState = (\<lambda> p st msgs crd. SyncMod_nextState p st msgs),
+    CnextState = (% p st msgs crd. SyncMod_nextState p st msgs),
     HOcommPerRd = SyncMod_commPerRd,
     HOcommGlobal = SyncMod_commGlobal,
     HOcommSchedule = SyncMod_commSchedule
 \<rparr>"
 
-lemma simp_nextState : "CnextState SyncMod_HOMachine = (\<lambda>p ss ms cr. SyncMod_nextState p ss ms)"
+lemma simp_nextState : "CnextState SyncMod_HOMachine = (% p ss ms cr. SyncMod_nextState p ss ms)"
 using SyncMod_HOMachine_def
 by (simp add: SyncMod_HOMachine_def)
 
 definition liveness where
-"liveness rho \<equiv> \<forall>p r. rho r p \<noteq> Aslept \<longrightarrow> (\<exists>rf sf. rho rf p = Active sf \<and> fire sf)"
+"liveness rho == ALL p r. rho r p ~= Aslept --> (EX rf sf. rho rf p = Active sf \<and> fire sf)"
 
 definition safety where
-"safety rho \<equiv> \<exists>c. \<forall>p rf ss sf. rho rf p = Active ss \<longrightarrow> (\<not> fire ss) \<longrightarrow> rho (Suc rf) p = Active sf \<longrightarrow> fire sf \<longrightarrow> (rf + c) mod k = 0"
+"safety rho == EX c. ALL p rf ss sf. rho rf p = Active ss -->
+                (~ fire ss) --> rho (Suc rf) p = Active sf --> fire sf --> (rf + c) mod k = 0"
 
 end
 end
